Stlc/SpecEquivalent.v
@@ -13,6 +13,22 @@ Lemma pctx_equiv_symm {Γ t₁ t₂ τ} :
   ⟪ Γ ⊢ t₁ ≃ t₂ : τ ⟫ → ⟪ Γ ⊢ t₂ ≃ t₁ : τ ⟫.
 Proof.
   unfold PCtxEquivalent.
-  intros equiv C τ' ty; split;  
+  intros equiv C τ' ty; split;
   apply (equiv C τ' ty).
+Qed.
+
+Definition PCtxEquivalentCtx (Γᵢ : Env) (C₁ C₂ : PCtx) (τᵢ τₒ : Ty) : Prop :=
+  ∀ t ,
+    ⟪ Γᵢ ⊢ t : τᵢ ⟫ →
+    (pctx_app t C₁)⇓ ↔ (pctx_app t C₂)⇓.
+Notation "⟪ ⊢ C₁ ≃ C₂ : Γᵢ , τᵢ → τₒ  ⟫" :=
+  (PCtxEquivalentCtx Γᵢ C₁ C₂ τᵢ τₒ)
+  (at level 0, Γᵢ  at level 98, C₁ at level 98, C₂ at level 98, τᵢ  at level 98, τₒ at level 98).
+
+Lemma pctx_equiv_ctx_symm {Γᵢ C₁ C₂ τᵢ τₒ} :
+  ⟪ ⊢ C₁ ≃ C₂ : Γᵢ , τᵢ → τₒ  ⟫ ->
+  ⟪ ⊢ C₂ ≃ C₁ : Γᵢ , τᵢ → τₒ  ⟫.
+Proof.
+  intros equiv C wsc; split;
+  apply (equiv C wsc).
 Qed.
