Utlc/SpecEquivalent.v
@@ -9,10 +9,27 @@ Notation "⟨  γ ⊢ t₁ ≃ t₂ ⟩" :=
   (PCtxEquivalent γ t₁ t₂)
   (at level 0, γ at level 10, t₁ at level 10, t₂ at level 10).
 
+Definition PCtxEquivalentCtx (γᵢ : Dom) (C₁ C₂: PCtx) : Prop :=
+  ∀ t,
+    wsUTm γᵢ t ->
+    (* ⟨ γᵢ ⊢ t ⟩ → *)
+    (pctx_app t C₁)⇓ ↔ (pctx_app t C₂)⇓.
+Notation "⟨ ⊢ C₁ ≃ C₂ : γᵢ → 0 ⟩" :=
+  (PCtxEquivalentCtx γᵢ C₁ C₂)
+  (at level 0, γᵢ at level 10, C₁ at level 10, C₂ at level 10).
+
 Lemma pctx_equiv_symm {γ t₁ t₂} :
   ⟨ γ ⊢ t₁ ≃ t₂ ⟩ → ⟨ γ ⊢ t₂ ≃ t₁ ⟩.
 Proof.
   unfold PCtxEquivalent.
-  intros equiv C wsc; split;  
+  intros equiv C wsc; split;
+  apply (equiv C wsc).
+Qed.
+
+Lemma pctx_equiv_ctx_symm {γᵢ C₁ C₂} :
+  ⟨ ⊢ C₁ ≃ C₂ : γᵢ → 0 ⟩ ->
+  ⟨ ⊢ C₂ ≃ C₁ : γᵢ → 0 ⟩.
+Proof.
+  intros equiv C wsc; split;
   apply (equiv C wsc).
 Qed.
