Compiler/ProtectConfine.v
@@ -693,7 +693,7 @@ Lemma protect_transp' {d w τ vs vu} :
 Proof.
   intros vr.
   destruct (protect_transp vr) as (vu' & vvu' & eu & vr').
-  refine (termrel_antired_star _ eu _); 
+  refine (termrel_antired_star _ eu _);
   eauto using valrel_in_termrel with eval.
 Qed.
 
@@ -705,6 +705,26 @@ Proof.
   assert (U.Value (protect τ)) by apply protect_Value.
   eapply (termrel_ectx' (Cs := S.phole) tr); inferContext; crush.
   intros; apply protect_transp'; crush.
+Qed.
+
+Lemma confine_transp' {d w τ vs vu} :
+  valrel d w (embed τ) vs vu →
+  termrel d w (embed τ) vs (U.app (confine τ) vu).
+Proof.
+  intros vr.
+  destruct (confine_transp vr) as (vu' & vvu' & eu & vr').
+  refine (termrel_antired_star _ eu _);
+  eauto using valrel_in_termrel with eval.
+Qed.
+
+Lemma confine_transp'' {d w τ ts tu} :
+  termrel d w (embed τ) ts tu →
+  termrel d w (embed τ) ts (U.app (confine τ) tu).
+Proof.
+  intros tr.
+  assert (U.Value (confine τ)) by apply confine_Value.
+  eapply (termrel_ectx' (Cs := S.phole) tr); inferContext; crush.
+  intros; apply confine_transp'; crush.
 Qed.
 
 (* Lemma confine_transp' {d w τ vs vu} : *)
@@ -725,4 +745,15 @@ Proof.
   unfold OpenLRN; crush; intros; crush; eauto using protect_closed.
   rewrite -> (wsClosed_invariant protect_closed γu).
   eapply protect_transp''; crush.
+Qed.
+
+
+Lemma confine_transp_open {d n τ ts tu Γ} :
+  ⟪ Γ ⊩ ts ⟦ d , n ⟧ tu : embed τ ⟫ →
+  ⟪ Γ ⊩ ts ⟦ d , n ⟧ U.app (confine τ) tu : embed τ ⟫.
+Proof.
+  destruct 1 as [ot lr].
+  unfold OpenLRN; crush; intros; crush; eauto using confine_closed.
+  rewrite -> (wsClosed_invariant confine_closed γu).
+  eapply confine_transp''; crush.
 Qed.
