FullAbstraction.v
@@ -29,11 +29,11 @@ Lemma equivalencePreservation {t₁ t₂ τ} :
   ⟨ 0 ⊢ compile τ t₁ ≃ compile τ t₂ ⟩.
 Proof.
   revert t₁ t₂ τ.
-  enough (∀ {t₁ t₂ τ}, 
+  enough (∀ {t₁ t₂ τ},
             ⟪ S.empty ⊢ t₁ : τ ⟫ →
             ⟪ S.empty ⊢ t₂ : τ ⟫ →
             ⟪ S.empty ⊢ t₁ ≃ t₂ : τ ⟫ →
-            ∀ {C}, ⟨ ⊢ C : 0 → 0 ⟩ →
+            ∀ {C}, WsPCtx 0 0 C →
                  U.Terminating (U.pctx_app (compile τ t₁) C) → U.Terminating (U.pctx_app (compile τ t₂) C)) as Hltor
       by (intros t₁ t₂ τ ty1 ty2 ceq;
           assert (⟪ S.empty ⊢ t₂ ≃ t₁ : τ ⟫)
@@ -45,7 +45,7 @@ Proof.
   destruct (U.Terminating_TerminatingN term) as [n termN]; clear term.
 
   assert (⟪ pempty ⊩ t₁ ⟦ dir_gt , S n ⟧ erase t₁ : embed τ ⟫) as lre₁
-      by (change pempty with (embedCtx (repEmulCtx pempty)); 
+      by (change pempty with (embedCtx (repEmulCtx pempty));
           eapply erase_correct;
           cbn; assumption).
   assert (⟪ pempty ⊩ S.app (inject (S (S n)) τ) t₁ ⟦ dir_gt , S n ⟧ U.app (protect τ) (erase t₁) : pEmulDV (S (S n)) precise ⟫) as lrpe₁
@@ -53,7 +53,7 @@ Proof.
           eauto using dwp_precise with arith).
   fold (compile τ t₁) in lrpe₁.
 
-  assert (⟪ ⊩ emulate_pctx (S (S n)) Cu ⟦ dir_gt , S n ⟧ Cu : 
+  assert (⟪ ⊩ emulate_pctx (S (S n)) Cu ⟦ dir_gt , S n ⟧ Cu :
               pempty , pEmulDV (S (S n)) precise → pempty , pEmulDV (S (S n)) precise ⟫) as lrem₁ by
       (change pempty with (toEmulDV (S (S n)) precise 0);
        eapply emulate_pctx_works; eauto using dwp_precise with arith).
@@ -81,7 +81,7 @@ Proof.
   destruct (S.Terminating_TerminatingN termS') as [m termSm']; clear termS'.
 
   assert (⟪ pempty ⊩ t₂ ⟦ dir_lt , S m ⟧ erase t₂ : embed τ ⟫) as lre₂
-      by (change pempty with (embedCtx (repEmulCtx pempty)); 
+      by (change pempty with (embedCtx (repEmulCtx pempty));
           eapply erase_correct;
           cbn; assumption).
   assert (⟪ pempty ⊩ S.app (inject (S (S n)) τ) t₂ ⟦ dir_lt , S m ⟧ U.app (protect τ) (erase t₂) : pEmulDV (S (S n)) imprecise ⟫) as lrpe₂
@@ -89,7 +89,7 @@ Proof.
           eauto using dwp_imprecise).
   fold (compile τ t₁) in lrpe₂.
 
-  assert (⟪ ⊩ emulate_pctx (S (S n)) Cu ⟦ dir_lt , S m ⟧ Cu : 
+  assert (⟪ ⊩ emulate_pctx (S (S n)) Cu ⟦ dir_lt , S m ⟧ Cu :
               pempty , pEmulDV (S (S n)) imprecise → pempty , pEmulDV (S (S n)) imprecise ⟫) as lrem₂ by
       (change pempty with (toEmulDV (S (S n)) imprecise 0);
        eapply emulate_pctx_works; eauto using dwp_imprecise).
@@ -111,4 +111,158 @@ Proof.
   eauto using equivalenceReflection, equivalencePreservation.
 Qed.
 
+Lemma equivalenceReflectionDF {C₁ C₂ τᵢ τₒ} :
+  ⟪ ⊢ C₁ : S.empty , τᵢ → S.empty , τₒ ⟫ ->
+  ⟪ ⊢ C₂ : S.empty , τᵢ → S.empty , τₒ ⟫ ->
+                                (* (⟨ ⊢ (compile_pctx τᵢ C₁) ≃ (compile_pctx τᵢ C₂) : dom Γᵢ → 0 ⟩). *)
+  PCtxEquivalentCtx 0 (compile_pctx τᵢ C₁) (compile_pctx τᵢ C₂) ->
+  ⟪ ⊢ C₁ ≃ C₂ : S.empty , τᵢ → τₒ  ⟫.
+Proof.
+  revert C₁ C₂ τᵢ τₒ.
+  enough (forall (C₁ C₂ : Stlc.SpecSyntax.PCtx) (τᵢ τₒ : Ty),
+            ⟪ ⊢ C₁ : S.empty, τᵢ → S.empty, τₒ ⟫ ->
+            ⟪ ⊢ C₂ : S.empty, τᵢ → S.empty, τₒ ⟫ ->
+            PCtxEquivalentCtx 0 (compile_pctx τᵢ C₁) (compile_pctx τᵢ C₂) ->
+            forall (t : Tm), ⟪ S.empty ⊢ t : τᵢ ⟫ -> Stlc.SpecEvaluation.Terminating (Stlc.SpecSyntax.pctx_app t C₁) ->
+              Stlc.SpecEvaluation.Terminating (Stlc.SpecSyntax.pctx_app t C₂)).
+  {
+    intros C₁ C₂ τᵢ τₒ tyC₁ tyC₂ seq t tyT.
+    split.
+    - intros termC₁.
+      eapply (H C₁ C₂ τᵢ τₒ tyC₁ tyC₂ seq t tyT termC₁).
+    - intros termC₂.
+      refine (H C₂ C₁ τᵢ τₒ tyC₂ tyC₁ _ t tyT termC₂).
+      eapply U.pctx_equiv_ctx_symm.
+      intuition.
+  }
+
+  intros C₁ C₂ τᵢ τₒ tyC₁ tyC₂ seq t tyT term.
+
+  destruct (S.Terminating_TerminatingN term) as [n termN]; clear term.
+  unfold compile_pctx in seq.
+
+  assert (⟪ ⊩ C₁ ⟦ dir_lt , S n ⟧ erase_pctx C₁ : pempty , embed τᵢ → pempty , embed τₒ ⟫) as lrC₁
+  by (change pempty with (embedCtx (repEmulCtx pempty));
+      eapply erase_ctx_correct; cbn; assumption).
+
+  assert (⟪ pempty ⊩ t ⟦ dir_lt , S n ⟧ U.app (confine τᵢ) (erase t) : embed τᵢ ⟫) as lrct
+  by (eapply confine_transp_open;
+      change pempty with (embedCtx S.empty);
+      eapply erase_correct;
+      assumption).
+
+  pose proof (proj2 lrC₁ _ _ lrct) as lrfull₁.
+
+  assert (U.Terminating (U.pctx_app (U.app (confine τᵢ) (erase t)) (erase_pctx C₁))) as termU₁
+  by (eapply (adequacy_lt lrfull₁ termN); eauto with arith).
+
+  assert (U.Terminating (U.pctx_app (U.app (confine τᵢ) (erase t)) (erase_pctx C₂))) as termU₂.
+  { specialize (seq (erase t)).
+    rewrite ?pctx_cat_app in seq.
+    eapply seq.
+    change 0 with (dom S.empty).
+    eapply (erase_scope _ _ _ tyT).
+    cbn. assumption.
+  }
+
+  destruct (U.Terminating_TerminatingN termU₂) as [n₂ termUN₂].
+  refine (adequacy_gt (n := S n₂) _ termUN₂ _); [|omega].
+
+  assert (⟪ ⊩ C₂ ⟦ dir_gt , S n₂ ⟧ erase_pctx C₂ : pempty , embed τᵢ → pempty , embed τₒ ⟫) as lrC₂
+  by (change pempty with (embedCtx (repEmulCtx pempty));
+      eapply erase_ctx_correct; cbn; assumption).
+
+  eapply (proj2 lrC₂).
+  eapply confine_transp_open.
+  change pempty with (embedCtx S.empty).
+  eapply erase_correct.
+  assumption.
+Qed.
+
+Lemma equivalencePreservationDF {C₁ C₂ τᵢ τₒ} :
+  ⟪ ⊢ C₁ : S.empty , τᵢ → S.empty , τₒ ⟫ ->
+  ⟪ ⊢ C₂ : S.empty , τᵢ → S.empty , τₒ ⟫ ->
+                                (* (⟨ ⊢ (compile_pctx τᵢ C₁) ≃ (compile_pctx τᵢ C₂) : dom Γᵢ → 0 ⟩). *)
+  ⟪ ⊢ C₁ ≃ C₂ : S.empty , τᵢ → τₒ  ⟫ ->
+  PCtxEquivalentCtx 0 (compile_pctx τᵢ C₁) (compile_pctx τᵢ C₂).
+Proof.
+  revert C₁ C₂ τᵢ τₒ.
+  enough (forall (C₁ C₂ : Stlc.SpecSyntax.PCtx) (τᵢ τₒ : Ty),
+            ⟪ ⊢ C₁ : S.empty, τᵢ → S.empty, τₒ ⟫ ->
+            ⟪ ⊢ C₂ : S.empty, τᵢ → S.empty, τₒ ⟫ ->
+            ⟪ ⊢ C₁ ≃ C₂ : S.empty, τᵢ → τₒ ⟫ ->
+            forall (t : UTm), wsUTm 0 t ->
+                         (pctx_app t (compile_pctx τᵢ C₁))⇓ → (pctx_app t (compile_pctx τᵢ C₂)) ⇓ ).
+  {
+    intros C₁ C₂ τᵢ τₒ tyC₁ tyC₂ seq t tyT.
+    split.
+    - intros termC₁.
+      eapply (H C₁ C₂ τᵢ τₒ tyC₁ tyC₂ seq t tyT termC₁).
+    - intros termC₂.
+      refine (H C₂ C₁ τᵢ τₒ tyC₂ tyC₁ _ t tyT termC₂).
+      eapply S.pctx_equiv_ctx_symm.
+      intuition.
+  }
+
+  intros C₁ C₂ τᵢ τₒ tyC₁ tyC₂ seq t tyT term.
+
+  destruct (U.Terminating_TerminatingN term) as [n termN]; clear term.
+  unfold compile_pctx in *.
+  rewrite ?U.pctx_cat_app in *.
+  cbn in *.
+
+  assert (⟪ ⊩ C₁ ⟦ dir_gt , S n ⟧ erase_pctx C₁ : pempty , embed τᵢ → pempty , embed τₒ ⟫) as lrC₁
+  by (change pempty with (embedCtx (repEmulCtx pempty));
+      eapply erase_ctx_correct; cbn; assumption).
+
+  assert (⟪ pempty ⊩ S.app (extract (S (S n)) τᵢ) (emulate (S (S n)) t) ⟦ dir_gt , S n ⟧ U.app (confine τᵢ) t : embed τᵢ ⟫) as lrct
+  by (eapply extract_works_open;
+      eauto using dwp_precise with arith;
+      change pempty with (toEmulDV (S (S n)) precise 0);
+      eapply emulate_works;
+      eauto using dwp_precise with arith;
+      assumption).
+
+  pose proof (proj2 lrC₁ _ _ lrct) as lrfull₁.
+
+
+  assert (S.Terminating (S.pctx_app (S.app (extract (S (S n)) τᵢ) (emulate (S (S n)) t)) C₁)) as termS₁
+  by (eapply (adequacy_gt lrfull₁ termN); eauto with arith).
+
+  assert (S.Terminating (S.pctx_app (S.app (extract (S (S n)) τᵢ) (emulate (S (S n)) t)) C₂)) as termS₂
+  by (eapply seq;
+    crushTyping;
+    eauto using extractT;
+    change S.empty with (toUVals (S (S n)) 0);
+    eapply emulate_T;
+    assumption).
+
+  destruct (S.Terminating_TerminatingN termS₂) as [n₂ termSN₂].
+  refine (adequacy_lt (n := S n₂) _ termSN₂ _); [|omega].
+
+  assert (⟪ ⊩ C₂ ⟦ dir_lt , S n₂ ⟧ erase_pctx C₂ : pempty , embed τᵢ → pempty , embed τₒ ⟫) as lrC₂
+  by (change pempty with (embedCtx (repEmulCtx pempty));
+      eapply erase_ctx_correct; cbn; assumption).
+
+  eapply lrC₂.
+  eapply extract_works_open.
+  - eauto using dwp_imprecise with arith.
+  - change pempty with (toEmulDV (S (S n)) imprecise 0).
+    eapply emulate_works; [|assumption].
+    eauto using dwp_imprecise with arith.
+Qed.
+
+Lemma fullAbstractionDF {C₁ C₂ : Stlc.SpecSyntax.PCtx} {τᵢ τₒ} :
+  ⟪ ⊢ C₁ : S.empty , τᵢ → S.empty , τₒ ⟫ ->
+  ⟪ ⊢ C₂ : S.empty , τᵢ → S.empty , τₒ ⟫ ->
+  ⟪ ⊢ C₁ ≃ C₂ : S.empty , τᵢ → τₒ  ⟫ ↔
+                                (* (⟨ ⊢ (compile_pctx τᵢ C₁) ≃ (compile_pctx τᵢ C₂) : dom Γᵢ → 0 ⟩). *)
+   PCtxEquivalentCtx 0 (compile_pctx τᵢ C₁) (compile_pctx τᵢ C₂).
+Proof.
+  intros.
+  split;
+  eauto using equivalencePreservationDF, equivalenceReflectionDF.
+Qed.
+
 Print Assumptions fullAbstraction.
+Print Assumptions fullAbstractionDF.
