UnaryFA.v
@@ -1,0 +1,116 @@
+Require Import Stlc.SpecTyping.
+Require Import Stlc.SpecEquivalent.
+Require Import Stlc.LemmasEvaluation.
+Require Import Stlc.LemmasTyping.
+Require Import Utlc.SpecEquivalent.
+Require Import Utlc.LemmasEvaluation.
+
+Require Import Compiler.Erase.
+Require Import Compiler.Compiler.
+Require Import Compiler.ProtectConfine.
+
+Require Import UVal.UVal.
+
+Require Import LogRel.PseudoType.
+Require Import LogRel.LemmasPseudoType.
+Require Import LogRel.LR.
+Require Import LogRel.LemmasLR.
+
+Require Import BackTrans.InjectExtract.
+Require Import BackTrans.UpgradeDowngrade.
+Require Import BackTrans.Emulate.
+
+Require Import Omega.
+
+Definition URobustlyDivergentCtx (γᵢ : Dom) (C : U.PCtx) : Prop :=
+  ∀ t,
+    wsUTm γᵢ t ->
+    (U.pctx_app t C) ⇑.
+
+Definition SRobustlyDivergentCtx (Γᵢ : Env) (C : S.PCtx) (τᵢ τₒ : Ty) : Prop :=
+  ∀ t ,
+    ⟪ Γᵢ ⊢ t : τᵢ ⟫ →
+    ¬ S.Terminating (S.pctx_app t C).
+
+
+Lemma equivalenceReflection1DF {C τᵢ τₒ} :
+  ⟪ ⊢ C : S.empty , τᵢ → S.empty , τₒ ⟫ ->
+  URobustlyDivergentCtx 0 (compile_pctx τᵢ C) ->
+  SRobustlyDivergentCtx S.empty C τᵢ τₒ.
+Proof.
+  intros tyC urd t tyT term.
+
+  destruct (S.Terminating_TerminatingN term) as [n termN]; clear term.
+  unfold compile_pctx in urd.
+
+  assert (⟪ ⊩ C ⟦ dir_lt , S n ⟧ erase_pctx C : pempty , embed τᵢ → pempty , embed τₒ ⟫) as lrC₁
+  by (change pempty with (embedCtx (repEmulCtx pempty));
+      eapply erase_ctx_correct; cbn; assumption).
+
+  assert (⟪ pempty ⊩ t ⟦ dir_lt , S n ⟧ U.app (confine τᵢ) (erase t) : embed τᵢ ⟫) as lrct
+  by (eapply confine_transp_open;
+      change pempty with (embedCtx S.empty);
+      eapply erase_correct;
+      assumption).
+
+  pose proof (proj2 lrC₁ _ _ lrct) as lrfull.
+
+  assert (U.Terminating (U.pctx_app (U.app (confine τᵢ) (erase t)) (erase_pctx C))) as termU
+  by (eapply (adequacy_lt lrfull termN); eauto with arith).
+
+  eapply (urd (erase t)).
+  - change 0 with (dom S.empty).
+    eapply (erase_scope _ _ _ tyT).
+  - rewrite U.pctx_cat_app.
+    cbn.
+    assumption.
+Qed.
+
+Lemma equivalencePreservation1DF {C τᵢ τₒ} :
+  ⟪ ⊢ C : S.empty , τᵢ → S.empty , τₒ ⟫ ->
+  SRobustlyDivergentCtx S.empty C τᵢ τₒ ->
+  URobustlyDivergentCtx 0 (compile_pctx τᵢ C).
+Proof.
+  intros tyC srd t tyT term.
+
+  destruct (U.Terminating_TerminatingN term) as [n termN]; clear term.
+  unfold compile_pctx in *.
+  rewrite ?U.pctx_cat_app in *.
+  cbn in *.
+
+ assert (⟪ ⊩ C ⟦ dir_gt , S n ⟧ erase_pctx C : pempty , embed τᵢ → pempty , embed τₒ ⟫) as lrC
+  by (change pempty with (embedCtx (repEmulCtx pempty));
+      eapply erase_ctx_correct; cbn; assumption).
+
+  assert (⟪ pempty ⊩ S.app (extract (S (S n)) τᵢ) (emulate (S (S n)) t) ⟦ dir_gt , S n ⟧ U.app (confine τᵢ) t : embed τᵢ ⟫) as lrct
+  by (eapply extract_works_open;
+      eauto using dwp_precise with arith;
+      change pempty with (toEmulDV (S (S n)) precise 0);
+      eapply emulate_works;
+      eauto using dwp_precise with arith;
+      assumption).
+
+  pose proof (proj2 lrC _ _ lrct) as lrfull.
+
+  assert (S.Terminating (S.pctx_app (S.app (extract (S (S n)) τᵢ) (emulate (S (S n)) t)) C)) as termS
+  by (eapply (adequacy_gt lrfull termN); eauto with arith).
+
+  refine (srd _ _ termS).
+  crushTyping.
+  - eapply extractT.
+  - change S.empty with (toUVals (S (S n)) 0).
+    eapply emulate_T.
+    assumption.
+Qed.
+
+Lemma fullAbstraction1DF {C : Stlc.SpecSyntax.PCtx} {τᵢ τₒ} :
+  ⟪ ⊢ C : S.empty , τᵢ → S.empty , τₒ ⟫ ->
+  SRobustlyDivergentCtx S.empty C τᵢ τₒ <->
+  URobustlyDivergentCtx 0 (compile_pctx τᵢ C).
+Proof.
+  intros.
+  split;
+  eauto using equivalencePreservation1DF, equivalenceReflection1DF.
+Qed.
+
+Print Assumptions fullAbstraction1DF.
